Finish refactoring to be in line with OTBN structure

riscv_model/spec/rv_ops.dfy
@@ -16,185 +16,179 @@ module rv_ops {
       
     datatype reg32_t = | Gpr(r: reg_index) // 32 32-bit registers, x0 is always zero
 
-// base integer instruction set, 32-bit
-datatype ins32I =
-| RV_LB(rd: Reg32, rs1: Reg32, oimm12: uint32)
-| RV_LH (rd: Reg32, rs1: Reg32, oimm12: uint32)
-| RV_LW (rd: Reg32, rs1: Reg32, oimm12: uint32)
-| RV_LBU (rd: Reg32, rs1: Reg32, oimm12: uint32)
-| RV_LHU (rd: Reg32, rs1: Reg32, oimm12: uint32)
+    type gprs_t = gprs : seq<uint32> | |gprs| == 32 witness *
 
-| RV_FENCE (pred: uint32, succ: uint32)
-| RV_FENCE_I
+      type mem_t = map<int, uint32>
 
-| RV_ADDI (rd: Reg32, rs1: Reg32, imm12: uint32) // sign extends, ignore overflow
-| RV_SLLI (rd: Reg32, rs1: Reg32, shamt6: uint32) // logical left shift
-| RV_SLTI (rd: Reg32, rs1: Reg32, imm12: uint32) // sign extend, 1 if rs1 (signed) < imm, else 0
-| RV_SLTIU (rd: Reg32, rs1: Reg32, imm12: uint32) // compare both vals as unsigned.
-| RV_XORI (rd: Reg32, rs1: Reg32, imm12: uint32)
-| RV_ORI (rd: Reg32, rs1: Reg32, imm12: uint32)
-| RV_ANDI (rd: Reg32, rs1: Reg32, imm12: uint32)
-| RV_SRLI (rd: Reg32, rs1: Reg32, shamt6: uint32) // logical right shift
-| RV_SRAI (rd: Reg32, rs1: Reg32, shamt6: uint32) // arithmetic right shift
+    predicate mem_addr_valid(mem: mem_t, addr: int)
+    {
+        && addr in mem
+    }
 
-| RV_AUIPC (rd: Reg32, oimm20: uint32)
+    predicate mem_addr_mapped(mem: mem_t, addr: int, value: uint32)
+    {
+        && mem_addr_valid(mem, addr)
+        && mem[addr] == value
+    }
 
-| RV_SB (rs1: Reg32, rs2: Reg32, simm12: uint32)
-| RV_SH (rs1: Reg32, rs2: Reg32, simm12: uint32)
-| RV_SW (rs1: Reg32, rs2: Reg32, simm12: uint32)
+    datatype state = state(
+        gprs: gprs_t, // 32-bit registers
+        mem: mem_t,
+        ok: bool)
+    {
+        function eval_reg32(r: reg32_t) : uint32
+        {
+            if r.index == 0 then 0
+            else gprs[r.index]
+        }
+    }
 
-| RV_ADD (rd: Reg32, rs1: Reg32, rs2: Reg32) // ignore overflow
-| RV_SUB (rd: Reg32, rs1: Reg32, rs2: Reg32) // ignore overflow
-| RV_SLL (rd: Reg32, rs1: Reg32, rs2: Reg32) // shift logical left by "lower 5 bits of rs2"
-| RV_SLT (rd: Reg32, rs1: Reg32, rs2: Reg32) // signed less than
-| RV_SLTU (rd: Reg32, rs1: Reg32, rs2: Reg32) // unsigned less than
-| RV_XOR (rd: Reg32, rs1: Reg32, rs2: Reg32) // bitwise
-| RV_SRL (rd: Reg32, rs1: Reg32, rs2: Reg32) // shift logical right by "lower 5 bits of rs2"
-| RV_SRA (rd: Reg32, rs1: Reg32, rs2: Reg32) // shift arithmetic right by "lower 5 bits of rs2"
-| RV_OR (rd: Reg32, rs1: Reg32, rs2: Reg32) // bitwise
-| RV_AND (rd: Reg32, rs1: Reg32, rs2: Reg32) // bitwise
+    predicate valid_state(s: state)
+    {
+        s.ok
+    }
+    
+    // base integer instruction set, 32-bit
+    datatype ins32I =
+    | RV_LB(rd: reg32_t, rs1: reg32_t, oimm12: uint32)
+    | RV_LH (rd: reg32_t, rs1: reg32_t, oimm12: uint32)
+    | RV_LW (rd: reg32_t, rs1: reg32_t, oimm12: uint32)
+    | RV_LBU (rd: reg32_t, rs1: reg32_t, oimm12: uint32)
+    | RV_LHU (rd: reg32_t, rs1: reg32_t, oimm12: uint32)
 
-| RV_LUI (rd: Reg32, imm20: uint32)
+    | RV_FENCE (pred: uint32, succ: uint32)
+    | RV_FENCE_I
 
-// | RV_BEQ (rs1: Reg32, rs2: Reg32, sbimm12: uint32)
-// | RV_BNE (rs1: Reg32, rs2: Reg32, sbimm12: uint32)
-// | RV_BLT (rs1: Reg32, rs2: Reg32, sbimm12: uint32)
-// | RV_BGE (rs1: Reg32, rs2: Reg32, sbimm12: uint32)
-// | RV_BLTU (rs1: Reg32, rs2: Reg32, sbimm12: uint32)
-// | RV_BGEU (rs1: Reg32, rs2: Reg32, sbimm12: uint32)
-// 
-// | RV_JALR (rd: Reg32, rs1: Reg32, oimm12: uint32)
-// | RV_JAL (rd: Reg32, jimm20: uint32)
+    | RV_ADDI (rd: reg32_t, rs1: reg32_t, imm12: uint32) // sign extends, ignore overflow
+    | RV_SLLI (rd: reg32_t, rs1: reg32_t, shamt6: uint32) // logical left shift
+    | RV_SLTI (rd: reg32_t, rs1: reg32_t, imm12: uint32) // sign extend, 1 if rs1 (signed) < imm, else 0
+    | RV_SLTIU (rd: reg32_t, rs1: reg32_t, imm12: uint32) // compare both vals as unsigned.
+    | RV_XORI (rd: reg32_t, rs1: reg32_t, imm12: uint32)
+    | RV_ORI (rd: reg32_t, rs1: reg32_t, imm12: uint32)
+    | RV_ANDI (rd: reg32_t, rs1: reg32_t, imm12: uint32)
+    | RV_SRLI (rd: reg32_t, rs1: reg32_t, shamt6: uint32) // logical right shift
+    | RV_SRAI (rd: reg32_t, rs1: reg32_t, shamt6: uint32) // arithmetic right shift
 
-// standard extension for integer mult and div, 32-bit
-datatype ins32M =
-| RV_MUL (rd: Reg32, rs1: Reg32, rs2: Reg32)
-| RV_MULH (rd: Reg32, rs1: Reg32, rs2: Reg32)
-| RV_MULHSU (rd: Reg32, rs1: Reg32, rs2: Reg32)
-| RV_MULHU (rd: Reg32, rs1: Reg32, rs2: Reg32)
-| RV_DIV (rd: Reg32, rs1: Reg32, rs2: Reg32)
-| RV_DIVU (rd: Reg32, rs1: Reg32, rs2: Reg32)
-| RV_REM (rd: Reg32, rs1: Reg32, rs2: Reg32)
-| RV_REMU (rd: Reg32, rs1: Reg32, rs2: Reg32)
+    | RV_AUIPC (rd: reg32_t, oimm20: uint32)
 
-// control and status register extension
-datatype ins32CSR =
-| RISC_ECALL
-| RISC_EBREAK
-| RISC_URET
-| RISC_SRET
-| RISC_MRET
-| RISC_WFI
-| RISC_SFENCE_VMA (rs1: Reg32, rs2: Reg32)
-| RISC_CSRRW (rd: Reg32, rs1: Reg32, csr12: uint32)
-| RISC_CSRRS (rd: Reg32, rs1: Reg32, csr12: uint32)
-| RISC_CSRRC (rd: Reg32, rs1: Reg32, csr12: uint32)
-| RISC_CSRRWI (rd: Reg32, zimm: uint32, csr12: uint32)
-| RISC_CSRRSI (rd: Reg32, zimm: uint32, csr12: uint32)
-| RISC_CSRRCI (rd: Reg32, zimm: uint32, csr12: uint32)
+    | RV_SB (rs1: reg32_t, rs2: reg32_t, simm12: uint32)
+    | RV_SH (rs1: reg32_t, rs2: reg32_t, simm12: uint32)
+    | RV_SW (rs1: reg32_t, rs2: reg32_t, simm12: uint32)
 
-datatype rv_ins32 = ins32I(ins: ins32I)| ins32M(ins: ins32M) | ins32CSR(ins: ins32CSR)
+    | RV_ADD (rd: reg32_t, rs1: reg32_t, rs2: reg32_t) // ignore overflow
+    | RV_SUB (rd: reg32_t, rs1: reg32_t, rs2: reg32_t) // ignore overflow
+    | RV_SLL (rd: reg32_t, rs1: reg32_t, rs2: reg32_t) // shift logical left by "lower 5 bits of rs2"
+    | RV_SLT (rd: reg32_t, rs1: reg32_t, rs2: reg32_t) // signed less than
+    | RV_SLTU (rd: reg32_t, rs1: reg32_t, rs2: reg32_t) // unsigned less than
+    | RV_XOR (rd: reg32_t, rs1: reg32_t, rs2: reg32_t) // bitwise
+    | RV_SRL (rd: reg32_t, rs1: reg32_t, rs2: reg32_t) // shift logical right by "lower 5 bits of rs2"
+    | RV_SRA (rd: reg32_t, rs1: reg32_t, rs2: reg32_t) // shift arithmetic right by "lower 5 bits of rs2"
+    | RV_OR (rd: reg32_t, rs1: reg32_t, rs2: reg32_t) // bitwise
+    | RV_AND (rd: reg32_t, rs1: reg32_t, rs2: reg32_t) // bitwise
 
-datatype code =
-| Ins32(ins: rv_ins32)
-| Block(block: codes)
-// | IfElse(ifCond: ifCond, ifTrue:code, ifFalse:code)
-| While(whileCond: whileCond, whileBody: code)
+    | RV_LUI (rd: reg32_t, imm20: uint32)
 
-datatype codes = CNil | va_CCons(hd: code, tl: codes)
+    // | RV_BEQ (rs1: reg32_t, rs2: reg32_t, sbimm12: uint32)
+    // | RV_BNE (rs1: reg32_t, rs2: reg32_t, sbimm12: uint32)
+    // | RV_BLT (rs1: reg32_t, rs2: reg32_t, sbimm12: uint32)
+    // | RV_BGE (rs1: reg32_t, rs2: reg32_t, sbimm12: uint32)
+    // | RV_BLTU (rs1: reg32_t, rs2: reg32_t, sbimm12: uint32)
+    // | RV_BGEU (rs1: reg32_t, rs2: reg32_t, sbimm12: uint32)
+    // 
+    // | RV_JALR (rd: reg32_t, rs1: reg32_t, oimm12: uint32)
+    // | RV_JAL (rd: reg32_t, jimm20: uint32)
 
-// todo
-datatype whileCond =
-    | RegCond(r: Reg32)
-    | ImmCond(c: uint32)
+    // standard extension for integer mult and div, 32-bit
+    datatype ins32M =
+    | RV_MUL (rd: reg32_t, rs1: reg32_t, rs2: reg32_t)
+    | RV_MULH (rd: reg32_t, rs1: reg32_t, rs2: reg32_t)
+    | RV_MULHSU (rd: reg32_t, rs1: reg32_t, rs2: reg32_t)
+    | RV_MULHU (rd: reg32_t, rs1: reg32_t, rs2: reg32_t)
+    | RV_DIV (rd: reg32_t, rs1: reg32_t, rs2: reg32_t)
+    | RV_DIVU (rd: reg32_t, rs1: reg32_t, rs2: reg32_t)
+    | RV_REM (rd: reg32_t, rs1: reg32_t, rs2: reg32_t)
+    | RV_REMU (rd: reg32_t, rs1: reg32_t, rs2: reg32_t)
 
-datatype state = state(
-    regs: map<Reg32, uint32>, // 32-bit registers
-    mem: map<int, uint32>,
-    ok: bool)
+    // control and status register extension
+    datatype ins32CSR =
+    | RISC_ECALL
+    | RISC_EBREAK
+    | RISC_URET
+    | RISC_SRET
+    | RISC_MRET
+    | RISC_WFI
+    | RISC_SFENCE_VMA (rs1: reg32_t, rs2: reg32_t)
+    | RISC_CSRRW (rd: reg32_t, rs1: reg32_t, csr12: uint32)
+    | RISC_CSRRS (rd: reg32_t, rs1: reg32_t, csr12: uint32)
+    | RISC_CSRRC (rd: reg32_t, rs1: reg32_t, csr12: uint32)
+    | RISC_CSRRWI (rd: reg32_t, zimm: uint32, csr12: uint32)
+    | RISC_CSRRSI (rd: reg32_t, zimm: uint32, csr12: uint32)
+    | RISC_CSRRCI (rd: reg32_t, zimm: uint32, csr12: uint32)
 
-predicate valid_state(s: state)
-{
-    (forall r :: r in s.regs)
-}
+    datatype rv_ins32 = ins32I(ins: ins32I)| ins32M(ins: ins32M) | ins32CSR(ins: ins32CSR)
 
-predicate IsUInt32(i: int) { 0 <= i < 0x1_0000_0000 }
+    predicate eval_ins32(xins: ins32, s: state, r: state)
+        {
+            if !s.ok then
+                !r.ok
+            else
+                r.ok && (valid_state(s) ==> valid_state(r))
+        }
 
-predicate ValidRegister32(regs: map<Reg32, uint32>, r: Reg32)
-{
-    r in regs
-}
+    /* control flow definitions */
 
-function eval_reg(regs: map<Reg32, uint32>, r: Reg32) : uint32
-{
-    if !ValidRegister32(regs, r) then 24 // TODO: better error message
-    else regs[r]
-}
+    datatype code =
+    | Ins32(ins: rv_ins32)
+    | Block(block: codes)
+    | While(whileCond: whileCond, whileBody: code)
+    | Comment(com: string)
 
-predicate ValidSourceRegister32(s: state, r: Reg32)
-{
-    ValidRegister32(s.regs, r)
-}
+    datatype codes =
+      | CNil
+      | va_CCons(hd: code, tl: codes)
 
-predicate ValidDestinationRegister32(s: state, r: Reg32)
-{
-    ValidRegister32(s.regs, r)
-}
+    // todo
+    datatype whileCond =
+        | RegCond(r: reg32_t)
+        | ImmCond(c: uint32)
 
-function eval_reg32(s: state, r: Reg32) : uint32
-{
-    if !ValidSourceRegister32(s, r) then
-        42
-    else
-        s.regs[r]
-}
 
-predicate evalIns32(ins: rv_ins32, s: state, r: state)
-{
-    if !s.ok then
-        !r.ok
-    else
-        r.ok && (valid_state(s) ==> valid_state(r))
-}
-
-predicate evalBlock(block: codes, s: state, r: state)
-{
-    if block.CNil? then
-        r == s
-    else
-        exists r': state :: evalCode(block.hd, s, r') && evalBlock(block.tl, r', r)
-}
-
-function eval_cond(s: state, wc: whileCond): nat
-    // requires ValidSourceRegister32(s, wc.r);
-    // requires IsUInt32(wc.c);
-{
-    match wc
-        case RegCond(r) => eval_reg(s.regs, r)
-        case ImmCond(c) => c
-}
-
-predicate evalWhile(c: code, n: nat, s: state, r: state)
-    decreases c, n
-{
-    if s.ok then
-        if n == 0 then
-            s == r
+predicate eval_block(block: codes, s: state, r: state)
+    {
+        if block.CNil? then
+            r == s
         else
-            exists loop_body_end: state :: evalCode(c, s, loop_body_end)
-                && evalWhile(c, n - 1, loop_body_end, r)
-    else
-        !r.ok
-}
+            exists r': state :: eval_code(block.hd, s, r') && eval_block(block.tl, r', r)
+    }
 
-predicate evalCode(c: code, s: state, r: state)
-    decreases c, 0
-{
-    match c
-        case Ins32(ins) => evalIns32(ins, s, r)
-        case Block(block) => evalBlock(block, s, r)
-        //case IfElse(cond, ifT, ifF) => evalIfElse(cond, ifT, ifF, s, r)
-        case While(cond, body) => evalWhile(body, eval_cond(s, cond), s, r)
-}
+    function eval_cond(s: state, wc: whileCond): nat
+    {
+        match wc 
+            case RegCond(r) => s.eval_reg32(r)
+            case ImmCond(c) => c
+    }
 
+    predicate eval_while(c: code, n: nat, s: state, r: state)
+        decreases c, n
+    {
+        if s.ok then
+            if n == 0 then
+                s == r
+            else
+                exists loop_body_end: state :: eval_code(c, s, loop_body_end)
+                    && eval_while(c, n - 1, loop_body_end, r)
+        else
+            !r.ok
+    }
+
+    predicate eval_code(c: code, s: state, r: state)
+        decreases c, 0
+    {
+        match c
+            case Ins32(ins) => eval_ins32(ins, s, r)
+            case Ins256(ins) => eval_ins256(ins, s, r)
+            case Block(block) => eval_block(block, s, r)
+            case While(cond, body) => eval_while(body, eval_cond(s, cond), s, r)
+            case Comment(com) => s == r
+    }
 }
